AbstractFormulas: Talk about local constants

Abstract_Formula.thy
@@ -6,39 +6,39 @@ imports
   Indexed_FSet
 begin
 locale Abstract_Formulas =
-  fixes freshenV :: "nat \<Rightarrow> 'var \<Rightarrow> 'var"
-  fixes rename :: "('var \<Rightarrow> 'var) \<Rightarrow> ('form \<Rightarrow> 'form)"
-  fixes fv :: "'form \<Rightarrow> 'var set"
+  fixes freshenLC :: "nat \<Rightarrow> 'var \<Rightarrow> 'var"
+  fixes renameLCs :: "('var \<Rightarrow> 'var) \<Rightarrow> ('form \<Rightarrow> 'form)"
+  fixes lconsts :: "'form \<Rightarrow> 'var set"
+  fixes closed :: "'form \<Rightarrow> bool"
   fixes subst :: "'subst \<Rightarrow> 'form \<Rightarrow> 'form"
-  fixes ran_fv :: "'subst \<Rightarrow> 'var set"
+  fixes subst_lconsts :: "'subst \<Rightarrow> 'var set"
   fixes anyP :: "'form"
-  assumes freshenV_eq_iff[simp]: "freshenV a v = freshenV a' v' \<longleftrightarrow> a = a' \<and> v = v'"
-  assumes fv_rename: "fv (rename p f) = p ` fv f"
-  assumes rename_closed: "fv f = {} \<Longrightarrow> rename p f = f"
-  assumes subst_closed: "fv f = {} \<Longrightarrow> subst s f = f"
-  assumes fv_subst: "fv (subst s f) \<subseteq> fv f \<union> ran_fv s"
-  assumes anyP_is_any': "\<exists> s. subst s (rename (freshenV a) anyP) = f"
+  assumes freshenLC_eq_iff[simp]: "freshenLC a v = freshenLC a' v' \<longleftrightarrow> a = a' \<and> v = v'"
+  assumes lconsts_renameLCs: "lconsts (renameLCs p f) = p ` lconsts f"
+  assumes rename_closed: "lconsts f = {} \<Longrightarrow> renameLCs p f = f"
+  assumes subst_closed: "closed f \<Longrightarrow> subst s f = f"
+  assumes closed_no_lconsts: "closed f \<Longrightarrow> lconsts f = {}"
+  assumes fv_subst: "lconsts (subst s f) \<subseteq> lconsts f \<union> subst_lconsts s"
+  assumes lconsts_anyP: "lconsts anyP = {}"
+  assumes anyP_is_any: "\<exists> s. subst s anyP = f"
 begin
   definition freshen :: "nat \<Rightarrow> 'form \<Rightarrow> 'form" where
-    "freshen n = rename (freshenV n)"
+    "freshen n = renameLCs (freshenLC n)"
 
-  lemma fv_freshen: "fv (freshen a f) = freshenV a ` fv f"
-    unfolding freshen_def by (rule fv_rename)
+  lemma lconsts_freshen: "lconsts (freshen a f) = freshenLC a ` lconsts f"
+    unfolding freshen_def by (rule lconsts_renameLCs)
 
-  lemma anyP_is_any: "\<exists> s. subst s (freshen a anyP) = f"
-    unfolding freshen_def by (rule anyP_is_any')
-
-  definition closed :: "'form \<Rightarrow> bool" where "closed f \<longleftrightarrow> fv f = {}"
-  lemma closed_fv: "closed f \<Longrightarrow> fv f = {}" unfolding closed_def by auto
-
+  lemma freshen_closed: "lconsts f = {} \<Longrightarrow> freshen a f = f"
+    unfolding freshen_def by (rule rename_closed)
+    
   lemma closed_eq:
     assumes "closed f1"
     assumes "closed f2"
     shows "subst s1 (freshen a1 f1) = subst s2 (freshen a2 f2) \<longleftrightarrow> f1 = f2"
   using assms
-    by (auto simp add: closed_def freshen_def fv_freshen subst_closed rename_closed)
+    by (auto simp add: closed_no_lconsts freshen_def lconsts_freshen subst_closed rename_closed)
 
-  lemma freshenV_range_eq_iff[simp]: "freshenV a v \<in> range (freshenV a') \<longleftrightarrow> a = a'"
+  lemma freshenLC_range_eq_iff[simp]: "freshenLC a v \<in> range (freshenLC a') \<longleftrightarrow> a = a'"
     by auto
 end
 
@@ -49,16 +49,18 @@ abbreviation plain_ant :: "'form \<Rightarrow> ('form, 'var) antecedent"
   where "plain_ant f \<equiv> Antecedent {||} f {}"
 
 locale Abstract_Rules =
-  Abstract_Formulas freshenV rename fv subst ran_fv anyP
-  for freshenV :: "nat \<Rightarrow> 'var \<Rightarrow> 'var"
-  and rename  :: "('var \<Rightarrow> 'var) \<Rightarrow> ('form \<Rightarrow> 'form)"
-  and fv :: "'form \<Rightarrow> 'var set"
+  Abstract_Formulas freshenLC renameLCs lconsts closed subst subst_lconsts anyP
+  for freshenLC :: "nat \<Rightarrow> 'var \<Rightarrow> 'var"
+  and renameLCs  :: "('var \<Rightarrow> 'var) \<Rightarrow> ('form \<Rightarrow> 'form)"
+  and lconsts :: "'form \<Rightarrow> 'var set"
+  and closed :: "'form \<Rightarrow> bool"
   and subst :: "'subst \<Rightarrow> 'form \<Rightarrow> 'form" 
-  and ran_fv :: "'subst \<Rightarrow> 'var set" 
+  and subst_lconsts :: "'subst \<Rightarrow> 'var set" 
   and anyP :: "'form" +
   fixes antecedent :: "'rule \<Rightarrow> ('form, 'var) antecedent list"
   fixes consequent :: "'rule \<Rightarrow> 'form list"
   and rules :: "'rule stream"
+  assumes no_empty_conclusions: "\<forall>xs\<in>sset rules. consequent xs \<noteq> []"
 begin
   definition f_antecedent :: "'rule \<Rightarrow> ('form, 'var) antecedent fset"
     where "f_antecedent r = fset_from_list (antecedent r)"
@@ -66,12 +68,13 @@ begin
 end
 
 locale Abstract_Task =
-  Abstract_Rules freshenV rename fv subst ran_fv anyP  antecedent consequent rules
-  for freshenV :: "nat \<Rightarrow> 'var \<Rightarrow> 'var"
-    and rename  :: "('var \<Rightarrow> 'var) \<Rightarrow> ('form \<Rightarrow> 'form)"
-    and fv :: "'form \<Rightarrow> 'var set"
+  Abstract_Rules freshenLC renameLCs lconsts closed subst subst_lconsts anyP  antecedent consequent rules
+  for freshenLC :: "nat \<Rightarrow> 'var \<Rightarrow> 'var"
+    and renameLCs  :: "('var \<Rightarrow> 'var) \<Rightarrow> ('form \<Rightarrow> 'form)"
+    and lconsts :: "'form \<Rightarrow> 'var set"
+    and closed :: "'form \<Rightarrow> bool"
     and subst :: "'subst \<Rightarrow> 'form \<Rightarrow> 'form" 
-    and ran_fv :: "'subst \<Rightarrow> 'var set" 
+    and subst_lconsts :: "'subst \<Rightarrow> 'var set" 
     and anyP :: "'form"
     and antecedent :: "'rule \<Rightarrow> ('form, 'var) antecedent list"
     and consequent :: "'rule \<Rightarrow> 'form list" 
@@ -80,7 +83,6 @@ locale Abstract_Task =
   fixes conclusions :: "'form list"
   assumes assumptions_closed: "\<And> a. a \<in> set assumptions \<Longrightarrow> closed a"
   assumes conclusions_closed: "\<And> c. c \<in> set conclusions \<Longrightarrow> closed c"
-  assumes no_empty_conclusions: "\<forall>xs\<in>sset rules. consequent xs \<noteq> []"
 begin
   definition ass_forms where "ass_forms = fset_from_list assumptions"
   definition conc_forms where "conc_forms = fset_from_list  conclusions"
@@ -95,13 +97,13 @@ begin
     assumes "pf \<in> set assumptions"
     shows "subst s (freshen a pf) = pf "
       using assms assumptions_closed 
-      by (simp add: closed_fv freshen_def rename_closed subst_closed)
+      by (simp add: closed_no_lconsts freshen_def rename_closed subst_closed)
 
   lemma subst_freshen_conclusions[simp]:
     assumes "pf \<in> set conclusions"
     shows "subst s (freshen a pf) = pf "
       using assms conclusions_closed 
-      by (simp add: closed_fv freshen_def rename_closed subst_closed)
+      by (simp add: closed_no_lconsts freshen_def rename_closed subst_closed)
 
   lemma subst_freshen_in_ass_formsI:
     assumes "pf \<in> set assumptions"
